I2SFI/Compiler.v
@@ -36,7 +36,7 @@ Definition prog_int := PMap.t ((list Procedure_id) *
 
 (******* Compiler Environment ************)
 
-Record compiler_env : Type := 
+Record compiler_env : Type :=
   {
     current_component : Component_id;
     next_label : N;
@@ -121,14 +121,14 @@ Definition get_SFI_code_address (cid : Component_id)
            (pid : Procedure_id)
            (offset : nat) : COMP (RiscMachine.address) :=
   do cenv <- get;
-    do sfiId <- get_sfiId cid;      
+    do sfiId <- get_sfiId cid;
     do cmap <- (lift (PMap.find cid (procId2slot cenv))
        "Missing component id in procId2slot"%string
           (CompEitherMonad.PosArg cid));
     do slotid <- (lift (PMap.find pid cmap)
        "Missing componentprocedure id in procId2slot"%string
        (CompEitherMonad.TwoPosArg cid pid));
-    ret (SFI.address_of sfiId slotid (N.of_nat offset)). 
+    ret (SFI.address_of sfiId slotid (N.of_nat offset)).
 
 Definition get_data_slotid (cid : Component_id) (bid : Block_id)
   : COMP (N) :=
@@ -139,17 +139,17 @@ Definition get_data_slotid (cid : Component_id) (bid : Block_id)
     lift (PMap.find bid cmap)
          "Missing block id in buffer2slot"%string
          (CompEitherMonad.TwoPosArg cid bid).
-      
+
 
 Definition get_SFI_data_address (cid : Component_id)
            (bid : Block_id)
            (offset :  Block.offset)
   : COMP (RiscMachine.address) :=
   do cenv <- get;
-    do psfiId <- get_sfiId cid;    
+    do psfiId <- get_sfiId cid;
      do pslotid <- get_data_slotid cid bid;
     ret (SFI.address_of psfiId pslotid (Z.to_N offset)).
-  
+
 
 (****************** Initial compiler environment *******************)
 
@@ -166,26 +166,26 @@ Definition exported_procs_labels (procs : PMap.t (PMap.t Intermediate.Machine.co
                    (fun i =>
                       match i with
                       | Intermediate.Machine.ILabel lbl => Pos.of_nat lbl
-                      | _ => 1%positive 
-                      end )                  
+                      | _ => 1%positive
+                      end )
                       (List.flat_map snd procs)
-                )                
+                )
                 1%positive) in
-  
+
   let component_exported_procs_labels cid pi procs : (PMap.t AbstractMachine.label) :=
       match PMap.find cid pi with
       | None => PMap.empty AbstractMachine.label
       | Some (exp_procs,_) =>
         let start_lbl := ((max_code_component_label procs) + 1)%N in
         let new_labels := List.map N.of_nat (List.seq (N.to_nat start_lbl)
-                                                      (List.length exp_procs)) in 
+                                                      (List.length exp_procs)) in
         PMapExtra.of_list (List.combine exp_procs
                              (List.combine
                                 (List.repeat cid (List.length exp_procs))
                                 new_labels))
       end in
   PMap.fold (fun cid procs_map acc =>
-          PMap.add 
+          PMap.add
                cid
                (
                  component_exported_procs_labels
@@ -200,7 +200,7 @@ Definition exported_procs_labels (procs : PMap.t (PMap.t Intermediate.Machine.co
 Fixpoint allocate_procedure_slots (procs : PMap.t (PMap.t Intermediate.Machine.code))
   : PMap.t (PMap.t N) :=
   PMapExtra.of_list (
-      List.map (fun '(cid,proc_map) =>               
+      List.map (fun '(cid,proc_map) =>
                   let pids := (List.map fst (PMap.elements proc_map)) in
                   (cid,
                    PMapExtra.of_list
@@ -223,15 +223,15 @@ Definition init_env (i_cid2SFIid : PMap.t N) (i_procId2slot : PMap.t (PMap.t N))
 (**************************** Slot allocation ************************************)
 
 (*
- * buffs: static buffers 
+ * buffs: static buffers
  * Updates environment: sets buffer2slot
- * Returns: memory with data slot 1 reserved for allocator and the static buffers 
+ * Returns: memory with data slot 1 reserved for allocator and the static buffers
  *          preallocated
  *)
 Fixpoint allocate_buffers (buffs :  (list (Component_id * (list (Block_id * (nat + list value))))))
   : COMP (RiscMachine.Memory.t) :=
   (* components with static buffers *)
-  let allocate_buffers1 buffs := 
+  let allocate_buffers1 buffs :=
       match buffs with
       | [] => ret RiscMachine.Memory.empty
       | (cid,lst) :: xs =>
@@ -239,14 +239,14 @@ Fixpoint allocate_buffers (buffs :  (list (Component_id * (list (Block_id * (nat
           do sfi_cid <- get_sfiId cid;
           match List.find (fun '(_,size) =>
                              match size with
-                             | inl nsz => 
+                             | inl nsz =>
                                Nat.ltb (N.to_nat SFI.SLOT_SIZE) nsz
                              | inr lst =>
                                Nat.ltb (N.to_nat SFI.SLOT_SIZE) (List.length lst)
                              end
                           ) lst
           with
-          | None => 
+          | None =>
             let blocks := PMapExtra.of_list
                             (List.combine (fst (List.split lst))
                                           (SFI.Allocator.allocate_data_slots
@@ -282,20 +282,20 @@ Fixpoint allocate_buffers (buffs :  (list (Component_id * (list (Block_id * (nat
          List.filter (fun id => (negb (List.existsb (Pos.eqb id) (List.map fst buffs))))
                      (List.map fst (PMap.elements (cid2SFIid cenv)))
        ) mem1.
-    
+
 
 Fixpoint init_buffers
          (mem : RiscMachine.Memory.t)
          (buffs :  (list (Component_id * (list (Block_id * (nat + list value))))))
   : COMP (RiscMachine.Memory.t) :=
 
-  let fix init_buffer mem sfi_cid slotid vals  : COMP (RiscMachine.Memory.t) := 
+  let fix init_buffer mem sfi_cid slotid vals  : COMP (RiscMachine.Memory.t) :=
       match vals with
       | nil => ret mem
       | (off,imval)::xs =>
         match imval with
         | Int n =>
-          init_buffer 
+          init_buffer
             (RiscMachine.Memory.set_value
                mem
                (SFI.address_of sfi_cid slotid (N.of_nat off)) n )
@@ -303,7 +303,7 @@ Fixpoint init_buffers
         | Ptr p =>
           let cid : Component_id := Pos.of_nat (Pointer.component p) in
           let bid : Block_id := Pos.of_nat (Pointer.block p) in
-          let offset := Pointer.offset p in    
+          let offset := Pointer.offset p in
           if (Z.ltb offset 0%Z)
           then fail "init_buffers negative offset for pointer" (TwoPosArg cid bid)
           else
@@ -312,7 +312,7 @@ Fixpoint init_buffers
               fail "init_buffers offset too large" (TwoPosArg cid bid)
             else
               do address <- get_SFI_data_address cid bid offset;
-              init_buffer 
+              init_buffer
                 (RiscMachine.Memory.set_value
                    mem
                    (SFI.address_of sfi_cid slotid (N.of_nat off))
@@ -321,7 +321,7 @@ Fixpoint init_buffers
         | _ => init_buffer mem sfi_cid slotid xs
         end
       end in
-                
+
   let fix init_buffers_comp mem cid (lst : (list (Block_id * (nat + list value))))
       : COMP (RiscMachine.Memory.t) :=
       match lst with
@@ -331,14 +331,14 @@ Fixpoint init_buffers
         | inl _ => ret mem
         | inr vals =>
           do cenv <- get;
-            do sfi_cid <- get_sfiId cid;           
+            do sfi_cid <- get_sfiId cid;
             do slotid <- get_data_slotid cid bid;
             do mem' <- init_buffer mem sfi_cid slotid
                (List.combine (List.seq 0 (List.length vals)) vals);
             init_buffers_comp mem' cid xs
         end
       end in
-  
+
   match buffs with
   | [] => ret mem
   | (cid,lst) :: xs =>
@@ -357,11 +357,11 @@ Definition sfi_top_address (rd : RiscMachine.Register.t)
       RiscMachine.Register.R_OR_DATA_MASK
     ; AbstractMachine.IConst
         (RiscMachine.to_value (SFI.OFFSET_BITS_NO + SFI.COMP_BITS_NO + 1%N))
-        rd                           
-    ; AbstractMachine.IBinOp (RiscMachine.ISA.ShiftLeft) 
+        rd
+    ; AbstractMachine.IBinOp (RiscMachine.ISA.ShiftLeft)
                              RiscMachine.Register.R_SFI_SP
                              rd
-                             rd                             
+                             rd
     ; AbstractMachine.IBinOp (RiscMachine.ISA.BitwiseOr)
                              rd
                              RiscMachine.Register.R_OR_DATA_MASK
@@ -375,7 +375,7 @@ Definition gen_push_sfi (cid : SFIComponent.id) : AbstractMachine.code :=
      (
         (sfi_top_address RiscMachine.Register.R_AUX1 cid)
           ++
-          [   
+          [
             AbstractMachine.IStore RiscMachine.Register.R_AUX1 RiscMachine.Register.R_RA
             ; AbstractMachine.IConst 1%Z RiscMachine.Register.R_AUX1
             ; AbstractMachine.IBinOp (RiscMachine.ISA.Addition)
@@ -393,14 +393,14 @@ Definition gen_pop_sfi : COMP(AbstractMachine.code) :=
       ret
         ( [
             AbstractMachine.ILabel lbl
-            ; AbstractMachine.IConst 1%Z RiscMachine.Register.R_RA 
+            ; AbstractMachine.IConst 1%Z RiscMachine.Register.R_RA
             ; AbstractMachine.IBinOp (RiscMachine.ISA.Subtraction)
                                      RiscMachine.Register.R_SFI_SP
                                      RiscMachine.Register.R_RA
                                      RiscMachine.Register.R_SFI_SP
           ]
             ++ (sfi_top_address RiscMachine.Register.R_RA cid)
-            ++ 
+            ++
             [
               AbstractMachine.ILoad RiscMachine.Register.R_RA
                                       RiscMachine.Register.R_RA
@@ -418,7 +418,7 @@ Definition gen_set_sfi_registers (cid : SFIComponent.id) : AbstractMachine.code 
     ; AbstractMachine.IConst code_mask RiscMachine.Register.R_T
   ].
 
-Definition compile_IConst 
+Definition compile_IConst
            (imval : Intermediate.Machine.imvalue)
            (reg : Intermediate.Machine.register)
   : COMP (AbstractMachine.code) :=
@@ -428,7 +428,7 @@ Definition compile_IConst
   | Intermediate.Machine.IPtr p =>
     let cid : Component_id := Pos.of_nat (Pointer.component p) in
     let bid : Block_id := Pos.of_nat (Pointer.block p) in
-    let offset := Pointer.offset p in    
+    let offset := Pointer.offset p in
     if (Z.ltb offset 0%Z)
     then fail "compile_IConst negative offset for pointer " (TwoPosArg cid bid)
     else
@@ -517,13 +517,13 @@ Definition compile_IAlloc (rp : Intermediate.Machine.register)
                                  r2
         (*   Load *r₂ -> r₁ *)
         ; AbstractMachine.ILoad r2  r1
-                                
+
         (*   Const r₂ <- 1 *)
         ; AbstractMachine.IConst (1%Z) r2
 
         (*   Binop r₁ <- r₁ + r₂ *)
         ; AbstractMachine.IBinOp (RiscMachine.ISA.Addition) r1  r2  r1
-                                 
+
         (*   Const r₂ <- Address of (s=1,cid,o=0)  *)
         ; AbstractMachine.IConst (RiscMachine.to_value (SFI.address_of cid 1%N 0%N))
                                  r2
@@ -533,14 +533,14 @@ Definition compile_IAlloc (rp : Intermediate.Machine.register)
       (* ; AbstractMachine.IStore r2  r1 *)
 
       ++ [
-        (* # calculate address (s=2*k+1,c,o=0) in r₁ *)      
+        (* # calculate address (s=2*k+1,c,o=0) in r₁ *)
         (*   Const r₂ <- N+S+1 *)
         AbstractMachine.IConst
             (RiscMachine.to_value (SFI.OFFSET_BITS_NO + SFI.COMP_BITS_NO + 1%N))
             r2
         (*   Binop r₁ <- r₁ << r₂ # k shift left (N+S+1) *)
         ; AbstractMachine.IBinOp (RiscMachine.ISA.ShiftLeft) r1  r2  r1
-                                 
+
         (*   Binop r₁ <- r₁ |  r_or_data_mask  *)
         ;  AbstractMachine.IBinOp (RiscMachine.ISA.BitwiseOr) r1
                                   RiscMachine.Register.R_OR_DATA_MASK r1
@@ -550,7 +550,7 @@ Definition compile_IAlloc (rp : Intermediate.Machine.register)
                                  r2
         (*   Load *r₂ -> r₂ *)
         ;  AbstractMachine.ILoad  r2  r2
-                                  
+
       ])%list.
 
 Definition compile_IReturn : COMP (AbstractMachine.code) :=
@@ -616,11 +616,11 @@ Fixpoint compile_instructions (ilist : Intermediate.Machine.code)
       ret (ai ++ res)
   end.
 
-(* Needs in environment: current_component and all the other fields initialized properly. *) 
-Definition compile_procedure 
+(* Needs in environment: current_component and all the other fields initialized properly. *)
+Definition compile_procedure
            (pid : Procedure_id)
            (code : Intermediate.Machine.code)
-           (interface :prog_int) 
+           (interface :prog_int)
   : COMP (AbstractMachine.code) :=
   (* if the procedure is exported then must add the sfi stuff*)
   do cenv <- get;
@@ -629,13 +629,13 @@ Definition compile_procedure
        "Can't find interface for component " (PosArg cid);
       let exported_procs := fst comp_interface in
       let is_exported := List.existsb (Pos.eqb pid) exported_procs in
-      do acode <- compile_instructions code; 
-        if is_exported then          
+      do acode <- compile_instructions code;
+        if is_exported then
             do proc_label <- get_proc_label cid pid;
             do sfiId <- get_sfiId cid;
             ret (
                 [AbstractMachine.IHalt; AbstractMachine.ILabel proc_label]
-                  ++ (gen_push_sfi sfiId) 
+                  ++ (gen_push_sfi sfiId)
                   ++ (gen_set_sfi_registers sfiId)
                   ++ acode )
         else
@@ -657,7 +657,7 @@ Definition check_component_labels (cid : Component_id)
                      | _ => acc'
                      end
                   )
-                  linstr acc                                                                   
+                  linstr acc
              )
              procs [] )
       in
@@ -666,13 +666,13 @@ Definition check_component_labels (cid : Component_id)
       then ret procs
       else fail " check_component_labels::label duplication in component" NoInfo
   in
-      
-  let check_procedure cid pid acode :=      
+
+  let check_procedure cid pid acode :=
       match acode with
       | _::(AbstractMachine.ILabel _)::_ => ret procs
       | _ => fail " check_component_labels::procedure label not found at offset" NoInfo
       end in
-  
+
   let fix check_component cid procs :=
       match procs with
       | nil => ret procs
@@ -696,7 +696,7 @@ Fixpoint compile_components (components : list (Component_id * PMap.t Intermedia
           do res <- compile_procedures xs interface;
           ret ((pid, compiled_proc)::res)
       end in
-  
+
   match components with
   | [] => ret []
   | (cid,procs)::xs =>
@@ -708,8 +708,8 @@ Fixpoint compile_components (components : list (Component_id * PMap.t Intermedia
   end.
 
 (*************** Code Alligment and ILabel Removal  *******************)
-(* 
-use crt to go over list 
+(*
+use crt to go over list
 - drop last ILabel from proc
 - if crt is not ILabel, copy and move on
 - if crt is ILabel
@@ -734,7 +734,7 @@ Definition layout_procedure
               (None,AbstractMachine.INop)
               (N.to_nat p))
         ++ [elt] in
-  
+
   (* accumulate labels *)
   let lcode1 :=
       List.map
@@ -743,7 +743,7 @@ Definition layout_procedure
            | nil => (None,i)
            | _ => (Some ll,i)
            end
-        )           
+        )
         (snd ( List.fold_left
             (fun acc elt =>
                let '(current_labels,lcode) := acc in
@@ -755,7 +755,7 @@ Definition layout_procedure
         )) in
   (* padding *)
       List.fold_left
-         (fun acc elt =>       
+         (fun acc elt =>
             match elt with
             | (None, i) => acc ++ [elt]
             | (Some ll, i) =>
@@ -768,7 +768,7 @@ Definition layout_procedure
                 else
                   padd acc elt
               | _ =>  padd acc elt
-                
+
               end
             end
          ) lcode1 nil.
@@ -789,12 +789,12 @@ Definition check_label_duplication (cid:Component_id)
          ) (PMap.elements procs) []) in
   Nat.eqb (List.length all_labels)
           (List.length (List.nodup label_eq_dec all_labels)).
-         
+
 
 Definition check_labeled_code ( labeled_code : (PMap.t (PMap.t AbstractMachine.lcode)))
   : COMP( (PMap.t (PMap.t AbstractMachine.lcode)) ) :=
   let check_procedure cid pid lcode :=
-      do l <- get_proc_label cid pid;        
+      do l <- get_proc_label cid pid;
         match lcode with
         | _::(Some [lbl],_)::_ => ret  labeled_code
         | _ => fail " check_labeled_code::procedure label not found at offset "
@@ -825,10 +825,10 @@ Definition check_labeled_code ( labeled_code : (PMap.t (PMap.t AbstractMachine.l
 (* acode: cid -> pid -> list of instr (labeled individually) *)
 Definition layout_code (acode : PMap.t (PMap.t AbstractMachine.code))
            (* association list of (cid,label) -> (pid, offset of label) *)
-  : (* new code with ILabel removed and INop introduced such that the 
+  : (* new code with ILabel removed and INop introduced such that the
        contraints are satisfied for jump targets *)
     COMP (PMap.t (PMap.t AbstractMachine.lcode)) :=
-  
+
   let fix layout_procedures cid  lst : COMP (PMap.t AbstractMachine.lcode) :=
         match lst with
         | [] => ret (PMap.empty AbstractMachine.lcode)
@@ -845,7 +845,7 @@ Definition layout_code (acode : PMap.t (PMap.t AbstractMachine.code))
       | (cid,procs_map)::xs =>
         do cenv <- get;
           do res_map <- aux xs;
-          do proc_res <- layout_procedures cid (PMap.elements procs_map); 
+          do proc_res <- layout_procedures cid (PMap.elements procs_map);
           ret (PMap.add cid proc_res res_map)
       end
   in
@@ -863,21 +863,21 @@ Definition index_of (lbl : AbstractMachine.label) (listing : AbstractMachine.lco
                     then
                       match crt_lbls with
                       | None => ((index+1)%nat,false)
-                      | Some llst => 
+                      | Some llst =>
                         if (List.existsb  (label_eqb lbl) llst)
                         then ((index)%nat,true)
                         else ((index+1)%nat,false)
                       end
                     else (index,found)) listing (0%nat,false)).
-  
-  
+
+
 Definition get_E (lcode : PMap.t (PMap.t AbstractMachine.lcode)) : COMP (Env.E) :=
-  
+
   let fix fold_procs cid procs_lst acc :=
       do cenv <- get;
       match procs_lst with
       | [] => ret acc
-      | (pid,lbl) :: xs =>        
+      | (pid,lbl) :: xs =>
         match PMap.find cid lcode with
         | None => fail "get_E did not find component in lcode" (PosArg cid)
         | Some procs_lmap =>
@@ -894,9 +894,9 @@ Definition get_E (lcode : PMap.t (PMap.t AbstractMachine.lcode)) : COMP (Env.E) 
           end
         end
       end in
-        
+
   let fix fold_comp (clist : list (Component_id*(PMap.t label)))
-          (acc : Env.E)  : COMP (Env.E) :=      
+          (acc : Env.E)  : COMP (Env.E) :=
       match clist with
       | [] => ret acc
       | (cid,pmap)::xs =>
@@ -916,13 +916,13 @@ Definition label2address (lc : PMap.t (PMap.t AbstractMachine.lcode))
       match list_instr with
       | [] => ret acc
       | (i,(None,_))::xs => fold_instr cid pid xs acc
-      | (i,(Some lbls,_))::xs => 
+      | (i,(Some lbls,_))::xs =>
         do address <- get_SFI_code_address cid pid i;
           fold_instr cid pid xs (acc++(List.combine
                                          lbls
                                          (List.repeat address (List.length lbls))))
       end in
-  
+
   let fix fold_procs cid procs_lst
           (acc : (PMap.t (list (AbstractMachine.label * RiscMachine.address)))) :=
       do cenv <- get;
@@ -936,9 +936,9 @@ Definition label2address (lc : PMap.t (PMap.t AbstractMachine.lcode))
            [];
           fold_procs cid xs (PMap.add pid res acc)
       end in
-        
+
   let fix fold_comp (clist : list (Component_id*(PMap.t AbstractMachine.lcode)))
-          (acc : (PMap.t (PMap.t (list (AbstractMachine.label * RiscMachine.address))))) :=      
+          (acc : (PMap.t (PMap.t (list (AbstractMachine.label * RiscMachine.address))))) :=
       match clist with
       | [] => ret acc
       | (cid,pmap)::xs =>
@@ -946,7 +946,7 @@ Definition label2address (lc : PMap.t (PMap.t AbstractMachine.lcode))
            (PMap.empty (list (AbstractMachine.label * RiscMachine.address)));
           fold_comp xs (PMap.add cid res acc)
       end in
-  
+
   fold_comp (PMap.elements lc)
               (PMap.empty (PMap.t (list (AbstractMachine.label * RiscMachine.address)))).
 
@@ -970,7 +970,7 @@ Definition  get_address_by_label
             (l2a :  (PMap.t (PMap.t (list (AbstractMachine.label * RiscMachine.address)))))
   : COMP (RiscMachine.address) :=
 
-  let ll := List.concat 
+  let ll := List.concat
               (List.flat_map (fun pmap => List.map snd (PMap.elements pmap))
                           (List.map snd (PMap.elements l2a)) (* list of PMap *))
   in match (List.find (fun '(l,a) => AbstractMachine.label_eqb l lbl) ll) with
@@ -1029,42 +1029,42 @@ Definition generate_instruction
   let (_,i) := li in
   match i with
   | AbstractMachine.INop => ret (RiscMachine.Memory.set_instr
-                                  mem0 address 
+                                  mem0 address
                                   RiscMachine.ISA.INop)
   | AbstractMachine.IConst v r => ret (RiscMachine.Memory.set_instr
-                                  mem0 address 
+                                  mem0 address
                                   (RiscMachine.ISA.IConst v r))
   | AbstractMachine.IMov r1 r2 => ret (RiscMachine.Memory.set_instr
-                                  mem0 address 
+                                  mem0 address
                                   (RiscMachine.ISA.IMov r1 r2))
   |  AbstractMachine.IBinOp op r1 r2 r3 => ret (RiscMachine.Memory.set_instr
-                                                 mem0 address 
+                                                 mem0 address
                                                  (RiscMachine.ISA.IBinOp op r1 r2 r3))
   | AbstractMachine.ILoad r1 r2 => ret (RiscMachine.Memory.set_instr
-                                  mem0 address 
+                                  mem0 address
                                   (RiscMachine.ISA.ILoad r1 r2))
   | AbstractMachine.IStore r1 r2 => ret (RiscMachine.Memory.set_instr
-                                  mem0 address 
+                                  mem0 address
                                   (RiscMachine.ISA.IStore r1 r2))
   | AbstractMachine.IJump r => ret (RiscMachine.Memory.set_instr
-                                  mem0 address 
+                                  mem0 address
                                   (RiscMachine.ISA.IJump r))
   | AbstractMachine.IBnz r lbl =>
     (* brach should be allowed only in the current procedure *)
     do target_address <- get_address cid pid lbl l2a;
       let branch_offset := ((Z.of_N target_address) - (Z.of_N address))%Z in
       ret (RiscMachine.Memory.set_instr
-             mem0 address 
+             mem0 address
              (RiscMachine.ISA.IBnz r branch_offset))
   | AbstractMachine.IJal lbl =>
     do new_address <- get_address_by_label lbl l2a;
       ret (RiscMachine.Memory.set_instr
-             mem0 address 
+             mem0 address
              (RiscMachine.ISA.IJal new_address))
   | AbstractMachine.IHalt => ret (RiscMachine.Memory.set_instr
-                                  mem0 address 
+                                  mem0 address
                                   RiscMachine.ISA.IHalt)
-    
+
   | _ => fail "generate_instruction"  NoInfo
   end.
 
@@ -1084,7 +1084,7 @@ Definition generate_procedure_code
         end in
     do res <- (aux linstrs (0%nat,mem0));
       ret (snd res).
-        
+
 Definition generate_component_code
            (cid : Component_id)
            (pmap : PMap.t lcode)
@@ -1121,16 +1121,16 @@ Definition convert_prog_interface (pi : Program.interface) : prog_int :=
     (elementsm pi) (PMap.empty  ((list Procedure_id) *
                                  (list (Component_id * Procedure_id)))).
 
-Definition convert_prog_buffers (buffers :  NMap (list (Block.id * (nat + list value))))
+Definition convert_prog_buffers (buffers : NMap {fmap Block.id -> nat + list value})
   : list (Component_id * (list (Block_id *  (nat + list value)))) :=
   List.fold_left
     (fun acc '(cid,l) =>
        (
-         (Pos.of_nat cid, List.map (fun '(bid,s) => (Pos.of_nat bid,s)) l)
+         (Pos.of_nat cid, List.map (fun '(bid,s) => (Pos.of_nat bid,s)) (elementsm l))
        )::acc
     )
     (elementsm buffers)
-    nil. 
+    nil.
 
 Definition convert_prog_procs (procs :  NMap (NMap Machine.code)) : PMap.t (PMap.t Machine.code) :=
   List.fold_left
@@ -1154,7 +1154,7 @@ Definition compile_program (ip : Intermediate.program) :=
   let cip := convert_prog_interface (Intermediate.prog_interface ip) in
   let buffs := convert_prog_buffers (Intermediate.prog_buffers ip) in
   let pr_progs := convert_prog_procs (Intermediate.prog_procedures ip) in
-  
+
   let cn := gen_cn cip in
   let cid2SFIid := List.fold_left
                      (fun acc '(cid,i)  =>
@@ -1168,21 +1168,21 @@ Definition compile_program (ip : Intermediate.program) :=
                         (fun m => List.map (fun '(_,(_,l)) => l) (PMap.elements m))
                         (List.map snd (PMap.elements procs_labels)))
                      1%N in
-  
+
   let procId2slot := allocate_procedure_slots pr_progs in
 
-  
+
   run (init_env cid2SFIid procId2slot procs_labels (max_label+1)%N)
         (
-         
+
           do data_mem' <- allocate_buffers buffs;
 
             do data_mem <- init_buffers data_mem' buffs;
-            
+
             do acode <- compile_components
                (PMap.elements pr_progs)
                cip;
-            
+
             do labeled_code  <- layout_code (PMapExtra.of_list acode);
 
             do e <- get_E labeled_code;
@@ -1192,17 +1192,17 @@ Definition compile_program (ip : Intermediate.program) :=
             match  (Intermediate.prog_main ip) with
             | None => fail "Missing main" NoInfo
             | Some (cid,pid) =>
-            
+
               do mem0 <- generate_comp0_memory (Pos.of_nat cid)
                  (Pos.of_nat pid) data_mem l2a;
 
                 do mem <- generate_code_memory labeled_code l2a mem0;
-            
+
                 ret {| TargetSFI.Machine.cn := (List.map Pos.to_nat cn);
                        TargetSFI.Machine.e := e;
                        TargetSFI.Machine.mem := mem;
                        TargetSFI.Machine.prog_interface := Intermediate.prog_interface ip;
                     |}
             end
-            
+
     ).
